introduce message invariant ValidLearnMessage

networkInvariantPrototypes/paxos/monotonic/messageInvariants.dfy
@@ -37,6 +37,7 @@ predicate MessageInv(c: Constants, v: Variables)
   && ValidAcceptMessage(c, v)
   // From Learner transitions
   && LearnerValidReceivedAccepts(c, v)
+  && ValidLearnMessage(c, v)
 }
 
 lemma InitImpliesMessageInv(c: Constants, v: Variables)
@@ -53,6 +54,7 @@ lemma MessageInvInductive(c: Constants, v: Variables, v': Variables)
   InvNextAcceptorValidPromised(c, v, v');
   InvNextValidPromiseMessage(c, v, v');
   InvNextValidAcceptMessage(c, v, v');
+  InvNextValidLearnMessage(c, v, v');
 }
 
 /***************************************************************************************
@@ -162,6 +164,15 @@ predicate LearnerValidReceivedAccepts(c: Constants, v: Variables)
     && acc in v.learners[idx].receivedAccepts[vb][i]
   ::
     Accept(vb, acc) in v.network.sentMsgs
+}
+
+predicate ValidLearnMessage(c: Constants, v: Variables)
+  requires v.WF(c)
+  requires ValidMessageSrc(c, v)
+{
+  forall learn | IsLearnMessage(v, learn)
+  :: 
+  (exists i :: LearnMessageMatchesHistory(c, v, learn, i))
 }
 
 
@@ -285,6 +296,38 @@ lemma InvNextValidAcceptMessage(c: Constants, v: Variables, v': Variables)
   }
 }
 
+// Because dafny can't handle alternating quantifiers
+lemma InvNextValidLearnMessage(c: Constants, v: Variables, v': Variables)
+  requires v.WF(c)
+  requires ValidMessageSrc(c, v)
+  requires ValidLearnMessage(c, v)
+  requires Next(c, v, v')
+  ensures ValidLearnMessage(c, v')
+{
+  forall learn | IsLearnMessage(v', learn)
+  ensures exists i :: LearnMessageMatchesHistory(c, v', learn, i)
+  {
+    var dsStep :| NextStep(c, v, v', dsStep);
+    var actor, msgOps := dsStep.actor, dsStep.msgOps;
+    if && dsStep.LearnerStep? 
+       && learn.lnr == actor 
+       && msgOps.send == Some(learn)
+    {
+      var lc, l, l' := c.learnerConstants[actor], v.learners[actor], v'.learners[actor];
+      var step :| LearnerHost.NextStep(lc, l, l', step, msgOps);
+      if step.LearnStep? {
+        var vb := VB(learn.val, learn.bal);
+        var i := |l'.receivedAccepts[vb]|-1;
+        assert LearnMessageMatchesHistory(c, v', learn, i);   // trigger
+      }
+    } else {
+      assert IsLearnMessage(v, learn);                        // trigger
+      var i :| LearnMessageMatchesHistory(c, v, learn, i);    // witness
+      assert LearnMessageMatchesHistory(c, v', learn, i);     // trigger
+    }
+  }
+}
+
 /***************************************************************************************
 *                                        Utils                                         *
 ***************************************************************************************/
@@ -339,6 +382,17 @@ predicate PromiseMessageMatchesHistory(c: Constants, v: Variables, prom: Message
   && 0 <= i < |v.acceptors[prom.acc].acceptedVB|
   && prom.bal == v.acceptors[prom.acc].promised[i]
   && prom.vbOpt == v.acceptors[prom.acc].acceptedVB[i]
+}
+
+predicate LearnMessageMatchesHistory(c: Constants, v: Variables, learn: Message, i: nat)
+  requires v.WF(c)
+  requires ValidMessageSrc(c, v)
+  requires IsLearnMessage(v, learn)
+{
+  && var vb := VB(learn.val, learn.bal);
+  && vb in v.learners[learn.lnr].receivedAccepts
+  && 0 <= i < |v.learners[learn.lnr].receivedAccepts[vb]|
+  && |v.learners[learn.lnr].receivedAccepts[vb][i]| >= c.f+1
 }
 
 }  // end module PaxosProof
